Add BinTree Insert/Sort

BinTree.dfy
@@ -1,10 +1,10 @@
-datatype BinTree = Node(BinTree, BinTree, int) | Leaf
+datatype BinTree = Node(BinTree, int, BinTree) | Leaf
 
 predicate binTree(node: BinTree)
 {
   match node
   case Leaf => true
-  case Node(left, right, x) =>
+  case Node(left, x, right) =>
       binTree(left) &&
       binTree(right) &&
       leqThan(left, x) &&
@@ -21,11 +21,24 @@ predicate geqThan(node: BinTree, num: int)
     forall y :: (y in Elements(node)) ==> y >= num
 }
 
+predicate sorted(a: array<int>, min: int, max: int)
+   requires a != null;
+   requires 0 <= min <= max < a.Length;
+   reads a;
+{
+  forall j, k :: min <= j < k <= max ==> a[j] <= a[k]
+}
+
+predicate sortedSeq(s: seq<int>)
+{
+  forall j, k :: 0 <= j < k < |s| ==> s[j] <= s[k]
+}
+
 function Elements(node: BinTree) : multiset<int>
 {
     match node
     case Leaf => multiset([])
-    case Node(left, right, x) =>
+    case Node(left, x, right) =>
         Elements(left) + Elements(right) + multiset{x}
 }
 
@@ -36,14 +49,76 @@ method Insert(node: BinTree, x: int) returns (ret: BinTree)
 {
     match node
     case Leaf =>
-        ret := Node(Leaf, Leaf, x);
-    case Node(left, right, data) =>
+        ret := Node(Leaf, x, Leaf);
+    case Node(left, data, right) =>
         if (x > data) {
             var newRight := Insert(right, x);
-            ret := Node(left, newRight, data);
+            ret := Node(left, data, newRight);
         }
         else {
             var newLeft := Insert(left, x);
-            ret := Node(newLeft, right, data);
+            ret := Node(newLeft, data, right);
         }
+}
+
+method Traverse(node: BinTree) returns (ret: seq<int>)
+  requires binTree(node);
+
+  ensures sortedSeq(ret);
+  ensures Elements(node) == multiset(ret);
+{
+  match node
+  case Leaf =>
+    ret := [];
+  case Node(left, data, right) =>
+    var seqLeft := Traverse(left);
+    var seqRight := Traverse(right);
+
+    assert forall i :: 0 <= i < |seqLeft| ==> seqLeft[i] in Elements(left);
+    assert forall i :: 0 <= i < |seqRight| ==> seqRight[i] in Elements(right);
+
+    ret := seqLeft + [data] + seqRight;
+}
+
+method Sort(a: array<int>)
+  modifies a;
+  requires a != null;
+  requires a.Length > 0;
+
+  ensures multiset(a[..]) == multiset(old(a[..]));
+  ensures sorted(a, 0, a.Length - 1);
+{
+  var i := 0;
+  var node := Leaf;
+
+  while (i < a.Length)
+  invariant 0 <= i <= a.Length;
+  invariant binTree(node);
+  invariant forall j :: 0 <= j <= a.Length ==> a[0..j] == old(a[0..j]);
+  invariant multiset(old(a[0..i])) == Elements(node);
+  {
+    node := Insert(node, a[i]);
+
+    i := i + 1;
+  }
+
+  assert old(a[0..(a.Length)]) == old(a[..]);
+
+  var sequence := Traverse(node);
+
+  assert |multiset(a[..])| == |sequence|;
+
+  i := 0;
+
+  while (i < |sequence|)
+  invariant 0 <= i <= |sequence|;
+  invariant 0 <= i <= a.Length;
+  invariant a[0..i] == sequence[0..i];
+  {
+    a[i] := sequence[i];
+
+    i := i + 1;
+  }
+
+  assert a[..] == sequence;
 }
